{
 "cells": [
  {
   "cell_type": "markdown",
   "id": "d41e837e-755e-4bb2-ba6d-379a6a36033a",
   "metadata": {},
   "source": [
    "### Lecture 1 Assignments"
   ]
  },
  {
   "cell_type": "markdown",
   "id": "659cc172-d8e9-4310-bade-e8c6454eba09",
   "metadata": {},
   "source": [
    "### Problem 1:\n",
    "Recall the definition of a rational number, denoted as $\\mathbb{Q}$. Prove that the Euler's number $e$ = $\\sum^{\\infty}_{k=0} \\frac{1}{k!} \\notin \\mathbb{Q}$. A factorial is defined as $k! = (k-1)(k-2)(k-3)...,\\forall k \\in \\mathbb{Z}^{+}$, note that $0! = 1$. Furthermore, a sum notation $\\sum^{\\infty}_{k=0} k = 0 + 1 + 2 + 3 + ... + ...$\n",
    "\n",
    "### Answer:\n",
    "Proof by contradiction<br>\n",
    "#### Step 1:\n",
    "Suppose $e$ is rational. This means it can be expressed as a fraction in its simplest form,\n",
    "\\begin{align*}\n",
    "e = \\frac{p}{q}\n",
    "\\end{align*}\n",
    "\n",
    "Where $p$ and $q$ are integers with no common factors, and $q \\neq 0$.\n",
    "\n",
    "#### Step 2:\n",
    "Consider the partial sum $S_{n}$ of the series up to $n$ terms:\n",
    "\\begin{align*}\n",
    "S_{n} = \\sum^{n}_{k=0} \\frac{1}{k!}\n",
    "\\end{align*}\n",
    "Define the remainder $R_{n}$ of the series as:\n",
    "\\begin{align*}\n",
    "R_{n} = e - S_{n} = \\sum^{\\infty}_{k=n-1} \\frac{1}{k!}\n",
    "\\end{align*}\n",
    "\n",
    "#### Step 3:\n",
    "The remainder $R_{n}$ can be bounded by: \n",
    "\\begin{align*}\n",
    "R_n < \\frac{(1}{(n+1)!} + \\frac{1}{(n+2)!} + \\cdots < \\frac{1}{(n+1)!} \\left(1 + \\frac{1}{n+1} + \\frac{1}{(n+1)^{2}} + \\cdots \\right)\n",
    "\\end{align*}\n",
    "\n",
    "The series in parentheses is a geometric series with sum less than 2, hence:\n",
    "\\begin{align*}\n",
    "R_n < \\frac{2}{(n+1)!}\n",
    "\\end{align*}\n",
    "\n",
    "#### Step 4:\n",
    "Choose $n$ such that $(n + 1)! > 2q$.\n",
    "\\begin{align*}\n",
    "R_n < \\frac{2}{(n+1)!} < \\frac{2}{2q} = \\frac{1}{q}\n",
    "\\end{align*}\n",
    "\n",
    "#### Step 5:\n",
    "Since $S_n$ is a sum of rational numbers, $S_n$ is rational.\n",
    "\\begin{align*}\n",
    "e=S_{n} + R_{n} = \\frac{a}{b} + R_{n}\n",
    "\\end{align*}\n",
    "\n",
    "for some integers $a$ and $b$. Multiplying both sides by $q$ gives:\n",
    "\\begin{align*}\n",
    "qe = qS_{n} + qR_{n} \n",
    "\\end{align*}\n",
    "\n",
    "Since $qe = p$ and $qS_{n}$ is an integer, let $qS_{n} = m$ where $m$ is an integer\n",
    "\\begin{align*}\n",
    "p = m + qR_{n} \n",
    "\\end{align*}\n",
    "\n",
    "Thus, $qR_{n} = p - m$ must be an integer.\n",
    "\n",
    "#### Step 6:\n",
    "Since $R_{n} < \\frac{1}{q}$, we have:\n",
    "\\begin{align*}\n",
    "0 < qR_{n} < 1\n",
    "\\end{align*}\n",
    "which means $qR_{n}$ is a positive number less than 1, contradicting the fact that $qR_{n}$ must be an integer.<br>\n",
    "\n",
    "Since our assumption that $e$ is rational leads to a contradiction, this means Euler's number $e$ is irrational:\n",
    "\\begin{align*}\n",
    "e \\notin \\mathbb{Q}\n",
    "\\end{align*}\n",
    "\n",
    "***\n",
    "### Problem 2:\n",
    "Prove Minkowski's Inequality for sums, $\\forall p > 1, (a_{k}, b_{k}) > 0$:\n",
    "\n",
    "\\begin{align*} \n",
    "        [ \\Sigma^{n}_{k=1}|a_{k} + b_{k}|^{p}]^\\frac{1}{p} \\leq [ \\Sigma^{n}_{k=1}|a_{k}|^{p}]^\\frac{1}{p} + [ \\Sigma^{n}_{k=1}|b_{k}|^{p}]^\\frac{1}{p}\n",
    "\\end{align*}\n",
    "\n",
    "### Answer:<br>\n",
    "#### Step 1:\n",
    "For $p > 1$, define $q$ by:\n",
    "\\begin{align*} \n",
    "q = \\frac{p}{p - 1}\n",
    "\\end{align*}\n",
    "\n",
    "Introduce the Hölder's Inequality\n",
    "\\begin{align*} \n",
    "\\Sigma^{n}_{k=1} |x_{k}y_{k}| \\leq (\\Sigma^{n}_{k=1}|x_{k}|^{p})^{\\frac{1}{p}}(\\Sigma^{n}_{k=1}|y_{k}|^{q})^\\frac{1}{q}\n",
    "\\end{align*}\n",
    "\n",
    "#### Step 2:\n",
    "Apply Hölder's Inequality\n",
    "\\begin{align*} \n",
    "    x_{k} = |a_{k} + b_{k}|^{p-1}\n",
    "\\end{align*}\n",
    "\\begin{align*}\n",
    "    y_{k} = |a_{k} + b_{k}|\n",
    "\\end{align*}\n",
    "\n",
    "#### Step 3:\n",
    "Use the triangle inequality on the term $|a_{k} + b_{k}|$ within $y_{k}$:\n",
    "\\begin{align*}\n",
    "|a_{k} + b_{k}| = |(a_{k} + b_{k}) - 0| \\leq |a_{k}| + |b_{k}|\n",
    "\\end{align*}\n",
    "\n",
    "Therefore:\n",
    "\\begin{align*}\n",
    "y_{k} = |(a_{k} + b_{k}) \\leq |a_{k}| + |b_{k}|\n",
    "\\end{align*}\n",
    "\n",
    "#### Step 4:\n",
    "Substitute into Hölder's Inequality\n",
    "\\begin{align*}\n",
    "\\Sigma^{n}_{k=1} |a_{k} + b_{k}|^{p} \\leq [\\Sigma^{n}_{k=1} |a_{k} + b_{k}|^{p-1} |a_{k} + b_{k}|]^\\frac{1}{p} \\cdot [\\Sigma^{n}_{k=1} (|a_{k}| + |b_{k}|)^{q}]^\\frac{1}{q}\n",
    "\\end{align*}\n",
    "\n",
    "#### Step 5:\n",
    "Simplify the terms:\n",
    "\\begin{align*}\n",
    "[\\Sigma^{n}_{k=1} (|a_{k}| + |b_{k}|)^{q}]^\\frac{1}{q} = [\\Sigma^{n}_{k=1} |a_{k}|^{q}]^\\frac{1}{q} + [\\Sigma^{n}_{k=1}  |b_{k}|^{q}]^\\frac{1}{q}\n",
    "\\end{align*}\n",
    "\n",
    "Put it all together:\n",
    "\\begin{align*}\n",
    "[\\Sigma^{n}_{k=1} |a_{k} + b_{k}|^{p}] \\leq [\\Sigma^{n}_{k=1} |a_{k} + b_{k}|^{p}]^\\frac{1}{p} \\cdot [\\Sigma^{n}_{k=1} |a_{k}|^{q}]^\\frac{1}{q} + [\\Sigma^{n}_{k=1}  |b_{k}|^{q}]^\\frac{1}{q}\n",
    "\\end{align*}\n",
    "\n",
    "Divide both sides by the common term on the left:\n",
    "\\begin{align*}\n",
    "1 \\leq [\\Sigma^{n}_{k=1} |a_{k}|^{q}]^\\frac{1}{q} + [\\Sigma^{n}_{k=1} |b_{k}|^{q}]^\\frac{1}{q}\n",
    "\\end{align*}\n",
    "\n",
    "Take the $pth$ power of both sides:\n",
    "\\begin{align*}\n",
    "1^{p} \\leq [\\Sigma^{n}_{k=1} |a_{k}|^{q}] + [\\Sigma^{n}_{k=1} |b_{k}|^{q}]\n",
    "\\end{align*}\n",
    "\n",
    "The key terms can be rewritten using the definition of q:\n",
    "\\begin{align*}\n",
    "[\\Sigma^{n}_{k=1} |a_{k}|^{q}] = [\\Sigma^{n}_{k=1} |a_{k}|^\\frac{p}{p-1}] \n",
    "\\end{align*}\n",
    "\n",
    "And after doing the same for the term with $b_{k}$, we raise both sides to the power of $\\frac{1}{p}$ to get:\n",
    "\\begin{align*}\n",
    "[ \\Sigma^{n}_{k=1}|a_{k} + b_{k}|^{p}]^\\frac{1}{p} \\leq [ \\Sigma^{n}_{k=1}|a_{k}|^{p}]^\\frac{1}{p} + [ \\Sigma^{n}_{k=1}|b_{k}|^{p}]^\\frac{1}{p}\n",
    "\\end{align*}\n",
    "\n",
    "\n",
    "***\n",
    "### Problem 3:\n",
    "Prove the triangle inequality $|x + y| \\leq |x| + |y|, \\forall (x,y) \\in \\mathbb{R}$\n",
    "### Answer:\n",
    "#### Case 1: $(x \\geq 0, y \\geq 0)$\n",
    "Both $x$ and $y$ are positive or zero. Since the sum of non-negative numbers is non-negative:\n",
    "\\begin{align*}\n",
    "(x + y) \\geq 0\n",
    "\\end{align*}\n",
    "Since the absolute value of non-negative numbers remains the same, we can write:\n",
    "\\begin{align*}\n",
    "|x + y| = x + y or |x| + |y| = x + y\n",
    "\\end{align*}\n",
    "Thus, $|x + y| = |x| + |y|$\n",
    "\n",
    "#### Case 2: $(x \\geq 0, y < 0)$\n",
    "$x$ is positive or zero and $y$ is negative. Since the absolute value of a negative number is positive:\n",
    "\\begin{align*}\n",
    "|x + y| \\leq x - y \n",
    "\\end{align*}\n",
    "Consider that $x$ and $y$ have opposite signs, $|x + (-y)| \\leq |x| + |y|$\n",
    "\n",
    "#### Case 3: $(x < 0, y \\geq 0)$\n",
    "Just like case 2, x and y have opposite signs.\n",
    "\\begin{align*}\n",
    "|x + y| \\leq -x + y \n",
    "\\end{align*}\n",
    "Thus, $|-x + y| \\leq |x| + |y|$\n",
    "\n",
    "#### Case 4: $(x < 0, y < 0)$\n",
    "Since both are non-negative, we can write:\n",
    "\\begin{align*}\n",
    "|x + y| = -(x + y) \n",
    "\\end{align*}\n",
    "\\begin{align*}\n",
    "|x| + |y| = -x -y \n",
    "\\end{align*}\n",
    "Therefore, $|x + y| = |x| + |y|$\n",
    "#### Conclusion:\n",
    "In all four cases, we arrived at an inequality that holds true\n",
    "***\n",
    "### Problem 4:\n",
    "Prove Sedrakayan's Lemma $\\forall u_{i}, v_{i} \\in \\mathbb{R}^{+}$:\n",
    "\\begin{align*}\n",
    "\\frac{(\\Sigma^{n}_{i=1} u_{i})^{2}}{\\Sigma^{n}_{i=1} v_{i}} \\leq \\Sigma^{n}_{i=1} \\frac{(u_{i})^{2}}{v_{i}}\n",
    "\\end{align*}\n",
    "### Answer:\n",
    "#### Step 1:\n",
    "The Cauchy-Schwarz inequality states that for any sequences of real numbers $a_{i}$ and $b_{i}$,\n",
    "\\begin{align*}\n",
    "(\\Sigma ^{n}_{i = 1} a_{i}b_{i})^{2} \\leq (\\Sigma ^{n}_{i = 1} a_{i}^{2})(\\Sigma ^{n}_{i = 1} b_{i}^{2})\n",
    "\\end{align*}\n",
    "Apply Cauchy-Schwarz inequality:\n",
    "\\begin{align*}\n",
    "a_{i} = \\frac{u_{i}}{\\sqrt{v_{i}}}   \\enspace and \\enspace   b_{i} = \\sqrt{v_{i}}\n",
    "\\end{align*}\n",
    "Now we get,\n",
    "\\begin{align*}\n",
    "(\\Sigma ^{n}_{i = 1} \\frac{u_{i}}{\\sqrt{v_{i}}}\\cdot \\sqrt{v_{i}})^{2} \\leq (\\Sigma ^{n}_{i = 1} (\\frac{u_{i}}{\\sqrt{v_{i}}})^{2})(\\Sigma ^{n}_{i = 1} (\\sqrt{v_{i}})^{2})\n",
    "\\end{align*}\n",
    "\n",
    "#### Step 2:\n",
    "Simplify the expressions:\n",
    "\\begin{align*}\n",
    "(\\Sigma ^{n}_{i = 1} \\frac{u_{i} \\sqrt{v_{i}}}{\\sqrt{v_{i}}})^{2} = (\\Sigma ^{n}_{i = 1}u_{i})^{2}\n",
    "\\end{align*}\n",
    "\\begin{align*}\n",
    "(\\Sigma ^{n}_{i = 1} (\\frac{u_{i}}{\\sqrt{v_{i}}})^{2})(\\Sigma ^{n}_{i = 1} (\\sqrt{v_{i}})^{2}) = (\\Sigma ^{n}_{i = 1} \\frac{u_{i}^{2}}{v_{i}})(\\Sigma ^{n}_{i = 1} v_{i})\n",
    "\\end{align*}\n",
    "\n",
    "#### Step 3:\n",
    "Combine the results:\n",
    "\\begin{align*}\n",
    "(\\Sigma ^{n}_{i = 1}u_{i})^{2} \\leq (\\Sigma ^{n}_{i = 1} \\frac{u_{i}^{2}}{v_{i}})(\\Sigma ^{n}_{i = 1} v_{i})\n",
    "\\end{align*}\n",
    "\n",
    "#### Step 4: \n",
    "Divide both sides by $\\Sigma ^{n}_{i = 1} v_{i}$ to get:\n",
    "\\begin{align*}\n",
    "\\frac{(\\Sigma ^{n}_{i = 1}u_{i})^{2}}{\\Sigma ^{n}_{i = 1} v_{i}} \\leq \\Sigma ^{n}_{i = 1} \\frac{(u_{i})^{2}}{v_{i}}\n",
    "\\end{align*}\n",
    "This completes the proof."
   ]
  },
  {
   "cell_type": "markdown",
   "id": "aa4a4a96-50c3-48b9-9e7b-7e76bf2e22c1",
   "metadata": {},
   "source": [
    "1. Consider the function $f(x) = 2x + 1, g(x) = 2y - 1, j(x) = |f(x) + g(x)|$, and $h(x) = j(x)^{2}$, show for the following inequality that:\n",
    "\n",
    "\\begin{align*}\n",
    "\\sqrt{|f(x)|^{2}} \\geq \\sqrt{h(x)} - \\sqrt{|g(x)|^{2}}, \\forall (x, y) \\in \\mathbb{Z}^{+}\n",
    "\\end{align*}\n",
    "\n",
    "### Answer:\n",
    "#### Step 1:\n",
    "Break it down:\n",
    "\\begin{align*}\n",
    "f(x) = 2x + 1\n",
    "\\end{align*}\n",
    "\\begin{align*}\n",
    "g(x) = 2y - 1\n",
    "\\end{align*}\n",
    "\\begin{align*}\n",
    "j(x) = |f(x) + g(x)| = |(2x + 1)+(2y - 1)| = |2x + 1 + 2y - 1| = |2(x+y)|\n",
    "\\end{align*}\n",
    "\\begin{align*}\n",
    "h(x) = j(x)^{2} = (2|x+y|)^{2} = 4(x+y)^2\n",
    "\\end{align*}\n",
    "\n",
    "#### Step 2:\n",
    "Substitute and evaluate:\n",
    "\\begin{align*}\n",
    "\\sqrt{|f(x)|^{2}} = \\sqrt{(2x + 1)^{2}} = |2x + 1|\n",
    "\\end{align*}\n",
    "\\begin{align*}\n",
    "\\sqrt{h(x)} = \\sqrt{4(x + y)^{2}} = 2|x + y|\n",
    "\\end{align*}\n",
    "\\begin{align*}\n",
    "\\sqrt{|g(x)|^{2}} = \\sqrt{(2y - 1)^{2}} = |2y - 1|\n",
    "\\end{align*}\n",
    "\n",
    "Combine the terms:\n",
    "\\begin{align*}\n",
    "|2x + 1| \\leq 2|x + y| - |2y - 1|\n",
    "\\end{align*}\n",
    "#### Step 3:\n",
    "#### Case: $x + y \\geq 1$:\n",
    "If $2x + 1 \\geq 0$ and $2y - 1 \\geq 0$, \n",
    "\\begin{align*}\n",
    "|2x + 1| = 2x + 1 \\enspace and \\enspace  |2y - 1| = 2y - 1\n",
    "\\end{align*}\n",
    "\\begin{align*}\n",
    "2x + 1 = \\geq 2(x + y) - (2y - 1)\n",
    "\\end{align*}\n",
    "\\begin{align*}\n",
    "2x + 1 = \\geq 2x + 1\n",
    "\\end{align*}\n",
    "This holds true as equality.\n",
    "#### Conclusion:\n",
    "The inequality holds true by considering the absolute values."
   ]
  },
  {
   "cell_type": "markdown",
   "id": "263ee8f9-8e4f-4297-b780-d102f4cdb947",
   "metadata": {},
   "source": [
    "2. Prove Sedrakayan's Lemma if $u_{i}, v_{i}$ are square roots of an even integer:\n",
    "\\begin{align*}\n",
    "\\frac{(\\Sigma^{n}_{i=1} u_{i})^{2}}{\\Sigma^{n}_{i=1} v_{i}} \\leq \\Sigma^{n}_{i=1} \\frac{(u_{i})^{2}}{v_{i}}\n",
    "\\end{align*}\n",
    "\n",
    "### Answer:\n",
    "#### Step 1:\n",
    "Cauchy-Schwarz Inequality:\n",
    "\\begin{align*}\n",
    "(\\Sigma ^{n}_{i = 1} a_{i}b_{i})^{2} \\leq (\\Sigma ^{n}_{i = 1} a_{i}^{2})(\\Sigma ^{n}_{i = 1} b_{i}^{2})\n",
    "\\end{align*}\n",
    "Apply Cauchy-Schwarz inequality:\n",
    "\\begin{align*}\n",
    "a_{i} = \\frac{u_{i}}{\\sqrt{v_{i}}}   \\enspace and \\enspace   b_{i} = \\sqrt{v_{i}}\n",
    "\\end{align*}\n",
    "Now we get,\n",
    "\\begin{align*}\n",
    "(\\Sigma ^{n}_{i = 1} \\frac{u_{i}}{\\sqrt{v_{i}}}\\cdot \\sqrt{v_{i}})^{2} \\leq (\\Sigma ^{n}_{i = 1} (\\frac{u_{i}}{\\sqrt{v_{i}}})^{2})(\\Sigma ^{n}_{i = 1} (\\sqrt{v_{i}})^{2})\n",
    "\\end{align*}\n",
    "#### Step 2:\n",
    "Simplify the expressions:\n",
    "\\begin{align*}\n",
    "(\\Sigma ^{n}_{i = 1} \\frac{u_{i} \\sqrt{v_{i}}}{\\sqrt{v_{i}}})^{2} = (\\Sigma ^{n}_{i = 1}u_{i})^{2}\n",
    "\\end{align*}\n",
    "\\begin{align*}\n",
    "(\\Sigma ^{n}_{i = 1} (\\frac{u_{i}}{\\sqrt{v_{i}}})^{2})(\\Sigma ^{n}_{i = 1} (\\sqrt{v_{i}})^{2}) = (\\Sigma ^{n}_{i = 1} \\frac{u_{i}^{2}}{v_{i}})(\\Sigma ^{n}_{i = 1} v_{i})\n",
    "\\end{align*}\n",
    "\n",
    "#### Step 3:\n",
    "Combine the results:\n",
    "\\begin{align*}\n",
    "(\\Sigma ^{n}_{i = 1}u_{i})^{2} \\leq (\\Sigma ^{n}_{i = 1} \\frac{u_{i}^{2}}{v_{i}})(\\Sigma ^{n}_{i = 1} v_{i})\n",
    "\\end{align*}\n",
    "\n",
    "#### Step 4: \n",
    "Divide both sides by $\\Sigma ^{n}_{i = 1} v_{i}$ to get:\n",
    "\\begin{align*}\n",
    "\\frac{(\\Sigma ^{n}_{i = 1}u_{i})^{2}}{\\Sigma ^{n}_{i = 1} v_{i}} \\leq \\Sigma ^{n}_{i = 1} \\frac{(u_{i})^{2}}{v_{i}}\n",
    "\\end{align*}\n",
    "This shows that the proof holds in this specific case."
   ]
  }
 ],
 "metadata": {
  "kernelspec": {
   "display_name": "Python 3 (ipykernel)",
   "language": "python",
   "name": "python3"
  },
  "language_info": {
   "codemirror_mode": {
    "name": "ipython",
    "version": 3
   },
   "file_extension": ".py",
   "mimetype": "text/x-python",
   "name": "python",
   "nbconvert_exporter": "python",
   "pygments_lexer": "ipython3",
   "version": "3.12.3"
  }
 },
 "nbformat": 4,
 "nbformat_minor": 5
}
